Updates in yul datatypes

evm_dialect.v
@@ -1,5 +1,12 @@
+Require Export FORYU.dialect.
 Require Export Coq.ZArith.ZArith.
 Global Open Scope Z_scope.
+Require Export Coq.Lists.List.
+Import ListNotations.
+Require Coq.Strings.HexString.
+Require Export Coq.Strings.String.
+
+
 
 
 Module U256.
@@ -72,79 +79,144 @@ Module EVM_opcode.
     Definition eqb (a b : t) : bool :=
       if eq_dec a b then true else false.
 
-    (*
-    Definition eqb (a b: EVM_opcode.t) : bool :=
-        match a,b with
-        | ADD,ADD => true
-        | MUL,MUL => true
-        | SUB,SUB => true
-        | DIV,DIV => true
-        | SDIV,SDIV => true
-        | MOD,MOD => true
-        | SMOD,SMOD => true
-        | ADDMOD,ADDMOD => true
-        | MULMOD,MULMOD => true
-        | EXP,EXP => true
-        | SIGNEXTEND,SIGNEXTEND => true
-        | LT,LT => true
-        | GT,GT => true
-        | SLT,SLT => true
-        | SGT,SGT => true
-        | EQ,EQ => true
-        | ISZERO,ISZERO => true
-        | AND,AND => true
-        | OR,OR => true
-        | XOR,XOR => true
-        | NOT,NOT => true
-        | BYTE,BYTE => true
-        | SHL,SHL => true
-        | SHR,SHR => true
-        | SAR,SAR => true
-        | ADDRESS,ADDRESS => true
-        | BALANCE,BALANCE => true
-        | ORIGIN,ORIGIN => true
-        | CALLER,CALLER => true
-        | CALLVALUE,CALLVALUE => true
-        | CALLDATALOAD,CALLDATALOAD => true
-        | CALLDATASIZE,CALLDATASIZE => true
-        | GASPRICE,GASPRICE => true
-        | EXTCODESIZE,EXTCODESIZE => true
-        | RETURNDATASIZE,RETURNDATASIZE => true
-        | EXTCODEHASH,EXTCODEHASH => true
-        | BLOCKHASH,BLOCKHASH => true
-        | COINBASE,COINBASE => true
-        | TIMESTAMP,TIMESTAMP => true
-        | NUMBER,NUMBER => true
-        | DIFFICULTY,DIFFICULTY => true
-        | GASLIMIT,GASLIMIT => true
-        | CHAINID,CHAINID => true
-        | SELFBALANCE,SELFBALANCE => true
-        | BASEFEE,BASEFEE => true
-        | CODESIZE,CODESIZE => true
-        | GAS, GAS => true
-        | JUMPI, JUMPI => true
-        | _,_ => false
-        end.
-    *)
 End EVM_opcode.
 
 
-Module Type DIALECT.
-  Parameter value_t : Type.
-  Parameter opcode_t : Type.
-  Parameter is_true_value: value_t -> bool.
-  Parameter is_false_value: value_t -> bool.
-  Parameter equal_values: value_t -> value_t -> bool.
-End DIALECT.
+Module EVMStorage.
+  (* From github.com/formal-land/coq-of-solidity/blob/develop/coq/CoqOfSolidity/simulations/CoqOfSolidity.v 
+  *)
+  Definition t : Set :=
+    U256.t -> U256.t.
+
+  Definition empty : t :=
+    fun _ => 0.
+
+  Definition update (storage : EVMStorage.t) (address value : U256.t) : EVMStorage.t :=
+    fun current_address =>
+      if address =? current_address then
+        value
+      else
+        storage current_address.
+End EVMStorage.
+
+
+Module EVMMemory.
+  (** From 
+      github.com/formal-land/coq-of-solidity/blob/develop/coq/CoqOfSolidity/simulations/CoqOfSolidity.v 
+  *)
+  (** We define the memory as a function instead of an explicit list as there can be holes in it. It
+      goes from addresses in [U256.t] to bytes represented as [Z]. *)
+  Definition t : Type :=
+    U256.t -> Z.
+
+  Definition empty : t :=
+    fun _ => 0.
+
+  (** Get the bytes from some memory from a start adress and for a certain length. *)
+  Definition get_bytes (memory : EVMMemory.t) (start length : U256.t) : list Z :=
+    List.map
+      (fun (i : nat) =>
+        let address : U256.t := start + Z.of_nat i in
+        memory address
+      )
+      (List.seq 0 (Z.to_nat length)).
+
+  Definition update_bytes (memory : EVMMemory.t) (start : U256.t) (bytes : list Z) : EVMMemory.t :=
+    fun address =>
+      let i : Z := address - start in
+      if andb (0 <=? i) (i <? Z.of_nat (List.length bytes)) then
+        List.nth_default 0 bytes (Z.to_nat i)
+      else
+        memory address.
+
+  Definition u256_as_bytes (value : U256.t) : list Z :=
+    List.map
+      (fun (i : nat) => Z.shiftr value (8 * (31 - Z.of_nat i)) mod 256)
+      (List.seq 0 32).
+
+  Fixpoint bytes_as_u256_aux (acc : Z) (bytes : list Z) : U256.t :=
+    match bytes with
+    | [] => acc
+    | byte :: bytes =>
+      bytes_as_u256_aux
+        (acc * 256 + byte)
+        bytes
+    end.
+
+  Definition bytes_as_u256 (bytes : list Z) : U256.t :=
+    bytes_as_u256_aux 0 bytes.
+
+  Lemma bytes_as_u256_bounds (bytes : list Z)
+      (H_bytes : List.Forall (fun byte => 0 <= byte < 256) bytes) :
+    0 <= bytes_as_u256 bytes < 2 ^ (8 * Z.of_nat (List.length bytes)).
+  Proof.
+  Admitted.
+
+  (*
+  Definition bytes_as_bytes (bytes : list Z) : list Nibble.byte :=
+    List.map
+      (fun (byte : Z) => Nibble.byte_of_N (Z.to_N byte))
+      bytes.
+  *)
+
+  Fixpoint hex_string_as_bytes (hex_string : string) : list Z :=
+    match hex_string with
+    | ""%string => []
+    | String.String a "" => [] (* this case is unexpected *)
+    | String.String a (String.String b rest) =>
+      match HexString.ascii_to_digit a, HexString.ascii_to_digit b with
+      | Some a, Some b =>
+        let byte := 16 * Z.of_N a + Z.of_N b in
+        byte :: hex_string_as_bytes rest
+      | _, _ => [] (* this case is unexpected *)
+      end
+    end.
+End EVMMemory.
+
+
+Module EVMMemorySegment.
+  (** List of bytes represented as Z. *)
+  Definition t : Type := list Z.
+  Definition empty : t := [].
+End EVMMemorySegment.
+
+
+Module EVMState.
+  Record t : Type := {
+    storage : EVMStorage.t;
+    memory: EVMMemory.t;
+    call_data_seg : EVMMemorySegment.t;
+    return_data_seg: EVMMemorySegment.t;
+  }.
+
+  Definition empty : t :=
+    {| 
+      storage := EVMStorage.empty;
+      memory := EVMMemory.empty;
+      call_data_seg := EVMMemorySegment.empty;
+      return_data_seg := EVMMemorySegment.empty;
+    |}.
+End EVMState.
+
+
+
 
 
 Module EVMDialect <: DIALECT.
   Definition value_t := U256.t.
   Definition opcode_t := EVM_opcode.t.
+  Definition dialect_state := EVMState.t.
+
   Definition is_true_value (v: value_t) : bool :=
     v =? 0.
   Definition is_false_value (v: value_t) : bool :=
     negb (is_true_value v).
   Definition equal_values (v1 v2: value_t) : bool :=
     v1 =? v2.
+
+  Definition execute_op_code (state: dialect_state) (op: opcode_t) (inputs: list value_t) : (dialect_state * Status.t) :=
+    (state, Status.Running). (* Placeholder for actual implementation *)
+
+  Definition empty_dialect_state : dialect_state :=
+    EVMState.empty.
 End EVMDialect.
