state.v
@@ -1,418 +1,53 @@
-Require Export Coq.ZArith.ZArith.
-Require Coq.Strings.HexString.
-Require Export Coq.Strings.String.
-Require Import List.
-Import ListNotations.
+Require Export FORYU.program.
 
-From Ltac2 Require Ltac2.
-Require Export Lia.
-From Hammer Require Export Tactics.
 
-Require Import FORYU.program.
+Module VariableAssignment(D: DIALECT).
+  (* Assignment from YUL variables to dialect values *)
+  Definition t := list (YULVariable.t * D.value_t).
 
-Global Open Scope string_scope.
-Global Open Scope Z_scope.
-(* Global Open Scope list_scope. *)
-
-(*
-
-Module U256.
-  Definition t := Z.
-
-  Module Valid.
-    Definition t (value : U256.t) : Prop :=
-      0 <= value < 2 ^ 256.
-  End Valid.
-
-  Definition of_bool (b : bool) : U256.t :=
-    if b then 1 else 0.
-End U256.
-
-Module Address.
-  (** This type is a synonym and acts mainly as documentation purpose. *)
-  Definition t : Set := U256.t.
-
-  Module Valid.
-    Definition t (address : Address.t) : Prop :=
-      0 <= address < 2 ^ 160.
-  End Valid.
-End Address.
-
-Module Environment.
-  Record t : Set := {
-    caller : U256.t;
-    (** Amount of wei sent to the current contract *)
-    callvalue : U256.t;
-    calldata : list Z;
-    (** The address of the contract. *)
-    address : U256.t;
-    (** The name of the current code that is being executed. *)
-    code_name : U256.t;
-  }.
-End Environment.
-
-Module BlockUnit.
-  (** The return value of a code block. *)
-  Inductive t : Set :=
-  (** The default value in case of success *)
-  | Tt
-  (** The instruction `break` was called *)
-  | Break
-  (** The instruction `continue` was called *)
-  | Continue
-  (** The instruction `leave` was called *)
-  | Leave.
-End BlockUnit.
-
-Module Result.
-  (** A wrapper for the result of an expression or a code block. We can either return a normal value
-      with [Ok], or a special instruction [Return] that will stop the execution of the contract. *)
-  Inductive t (A : Set) : Set :=
-  | Ok (output : A)
-  | Return (p s : U256.t)
-  | Revert (p s : U256.t).
-  Arguments Ok {_}.
-  Arguments Return {_}.
-  Arguments Revert {_}.
-
-  Definition map {A B : Set} (f : A -> B) (value : t A) : t B :=
-    match value with
-    | Ok output => Ok (f output)
-    | Return p s => Return p s
-    | Revert p s => Revert p s
+  Definition empty : t := nil.
+  Definition assign (assignments : t) (var : YULVariable.t) (value : D.value_t) : t :=
+    (var, value) :: assignments.
+  Definition get (assignments : t) (var : YULVariable.t) : option D.value_t :=
+    match List.find (fun '(v,_) => YULVariable.eqb v var) assignments with
+    | None => None
+    | Some (_, value) => Some value
     end.
-End Result.
+End VariableAssignment.
 
-Module Memory.
-  (** We define the memory as a function instead of an explicit list as there can be holes in it. It
-      goes from addresses in [U256.t] to bytes represented as [Z]. *)
-  Definition t : Set :=
-    U256.t -> Z.
 
-  Definition empty : t :=
-    fun _ => 0.
+Module CallStack(D: DIALECT).
+  (* Stack of variable assignments for the calling functions *)
+  Module VariableAssignmentD := VariableAssignment(D).
+  Definition t := list VariableAssignmentD.t.
 
-  (** Get the bytes from some memory from a start adress and for a certain length. *)
-  Definition get_bytes (memory : Memory.t) (start length : U256.t) : list Z :=
-    List.map
-      (fun (i : nat) =>
-        let address : U256.t := start + Z.of_nat i in
-        memory address
-      )
-      (List.seq 0 (Z.to_nat length)).
-
-  Definition update_bytes (memory : Memory.t) (start : U256.t) (bytes : list Z) : Memory.t :=
-    fun address =>
-      let i : Z := address - start in
-      if andb (0 <=? i) (i <? Z.of_nat (List.length bytes)) then
-        List.nth_default 0 bytes (Z.to_nat i)
-      else
-        memory address.
-
-  Definition u256_as_bytes (value : U256.t) : list Z :=
-    List.map
-      (fun (i : nat) => Z.shiftr value (8 * (31 - Z.of_nat i)) mod 256)
-      (List.seq 0 32).
-
-  Fixpoint bytes_as_u256_aux (acc : Z) (bytes : list Z) : U256.t :=
-    match bytes with
-    | [] => acc
-    | byte :: bytes => bytes_as_u256_aux (acc * 256 + byte) bytes
+  Definition empty : t := nil.
+  Definition push (call_stack : t) (assignments : VariableAssignmentD.t) : t :=
+    assignments :: call_stack.
+  Definition pop (call_stack : t) : t :=
+    match call_stack with
+    | nil => nil
+    | _ :: rest => rest
     end.
-
-  Definition bytes_as_u256 (bytes : list Z) : U256.t :=
-    bytes_as_u256_aux 0 bytes.
-
-  Lemma bytes_as_u256_bounds (bytes : list Z)
-      (H_bytes : List.Forall (fun byte => 0 <= byte < 256) bytes) :
-    0 <= bytes_as_u256 bytes < 2 ^ (8 * Z.of_nat (List.length bytes)).
-  Proof.
-  Admitted.
-
-  (* Definition bytes_as_bytes (bytes : list Z) : list Nibble.byte :=
-    List.map
-      (fun (byte : Z) => Nibble.byte_of_N (Z.to_N byte))
-      bytes.
-  *)
-
-  Fixpoint hex_string_as_bytes (hex_string : string) : list Z :=
-    match hex_string with
-    | "" => []
-    | String.String a "" => [] (* this case is unexpected *)
-    | String.String a (String.String b rest) =>
-      match HexString.ascii_to_digit a, HexString.ascii_to_digit b with
-      | Some a, Some b =>
-        let byte := 16 * Z.of_N a + Z.of_N b in
-        byte :: hex_string_as_bytes rest
-      | _, _ => [] (* this case is unexpected *)
-      end
-    end.
-End Memory.
-
-Module Storage.
-  (** Each slot in the storage is a word. This is different from [Memory.t] where it is only
-      bytes. *)
-  Definition t : Set :=
-    U256.t -> U256.t.
-
-  Definition empty : t :=
-    fun _ => 0.
-
-  Definition update (storage : Storage.t) (address value : U256.t) : Storage.t :=
-    fun current_address =>
-      if address =? current_address then
-        value
-      else
-        storage current_address.
-End Storage.
-
-Module CallStack.
-  (** The list of functions that were called with their corresponding parameters. This is for
-      debugging purpose only, and does not exist in the semantics of Yul. *)
-  Definition t : Set :=
-    list (string * list (string * U256.t)).
 End CallStack.
 
-Module Dict.
-  Definition t (K V : Set) : Set :=
-    list (K * V).
 
-  Module Valid.
-    Definition t {K V : Set} (P_K : K -> Prop) (P_V : V -> Prop) (dict : Dict.t K V) : Prop :=
-      List.Forall (fun '(k, v) => P_K k /\ P_V v) dict.
-  End Valid.
-
-  Module Eq.
-    Class C (A : Set) : Set :=
-      eqb : A -> A -> bool.
-
-    Global Instance IZ : C Z :=
-      Z.eqb.
-
-    Global Instance IString : C string :=
-      String.eqb.
-
-    Global Instance ITuple2 {A B : Set} `{C A} `{C B} : C (A * B) :=
-      fun '(a1, b1) '(a2, b2) =>
-        andb (eqb a1 a2) (eqb b1 b2).
-  End Eq.
-
-  Fixpoint get {K V : Set} `{Eq.C K} (dict : t K V) (key : K) : option V :=
-    match dict with
-    | [] => None
-    | (current_key, current_value) :: dict =>
-      if Eq.eqb key current_key then
-        Some current_value
-      else
-        get dict key
-    end.
-
-  Lemma get_is_valid {K V : Set} `{Eq.C K} P_K P_V (dict : t K V) (key : K)
-      (H_dict : Valid.t P_K P_V dict) :
-    match get dict key with
-    | None => True
-    | Some value => P_V value
-    end.
-  Proof.
-    induction dict as [|(current_key, current_value) dict IH]; cbn; trivial.
-    sauto q: on.
-  Qed.
-
-  Lemma get_map_commut {K V1 V2 : Set} `{Eq.C K}
-      (dict : t K V1) (key : K) (f : V1 -> V2) :
-    match get dict key with
-    | None => None
-    | Some value => Some (f value)
-    end =
-    get (List.map (fun '(k, v) => (k, f v)) dict) key.
-  Proof.
-    induction dict as [|(current_key, current_value) dict IH]; cbn; trivial.
-    hauto q: on.
-  Qed.
-
-  Definition declare {K V : Set} (dict : t K V) (key : K) (value : V) : t K V :=
-    (key, value) :: dict.
-
-  Fixpoint assign_function {K V : Set} `{Eq.C K}
-      (dict : t K V) (key : K) (f : V -> V) :
-      option (t K V) :=
-    match dict with
-    | [] => None
-    | ((current_key, current_value) as entry) :: dict =>
-      if Eq.eqb current_key key then
-        Some ((current_key, f current_value) :: dict)
-      else
-        match assign_function dict key f with
-        | None => None
-        | Some dict => Some (entry :: dict)
-        end
-    end.
-
-  Definition assign {K V : Set} `{Eq.C K} (dict : t K V) (key : K) (value : V) :
-      option (t K V) :=
-    assign_function dict key (fun _ => value).
-
-  Fixpoint declare_or_assign_function {K V : Set} `{Eq.C K}
-      (dict : t K V) (key : K) (f : option V -> V) :
-      t K V :=
-    match dict with
-    | [] => [(key, f None)]
-    | ((current_key, current_value) as entry) :: dict =>
-      if Eq.eqb current_key key then
-        (key, f (Some current_value)) :: dict
-      else
-        entry :: declare_or_assign_function dict key f
-    end.
-
-  Definition declare_or_assign {K V : Set} `{Eq.C K}
-      (dict : t K V) (key : K) (value : V) :
-      t K V :=
-    declare_or_assign_function dict key (fun _ => value).
-
-  Lemma declare_or_assign_is_valid {K V : Set} `{Eq.C K} P_K P_V
-      (dict : t K V) (key : K) (value : V)
-      (H_dict : Valid.t P_K P_V dict)
-      (H_key : P_K key)
-      (H_value : P_V value) :
-    Valid.t P_K P_V (declare_or_assign dict key value).
-  Proof.
-    induction dict as [|(current_key, current_value) dict IH]; cbn; sauto q: on.
-  Qed.
-
-  Lemma declare_or_assign_map_commut {K V1 V2 : Set} `{Eq.C K}
-      (dict : t K V1) (key : K) (value : V1) (f : V1 -> V2) :
-    List.map (fun '(k, v) => (k, f v)) (declare_or_assign dict key value) =
-    declare_or_assign (List.map (fun '(k, v) => (k, f v)) dict) key (f value).
-  Proof.
-    induction dict as [|(current_key, current_value) dict IH]; cbn; trivial.
-    hauto q: on.
-  Qed.
-End Dict.
-
-Module Account.
-  Record t : Set := {
-    balance : U256.t;
-    nonce: Z;
-    code : U256.t;
-    (** When calling a constructor the parameters are concatenated to the code. We represent them
-        here. *)
-    codedata : list Z;
-    storage : Storage.t;
-    immutables : Dict.t U256.t U256.t;
-  }.
-End Account.
-
-Module Stack.
-  Definition t : Set :=
-    list Locals.t.
-
-  Definition open_scope (stack : t) : t :=
-    [] :: stack.
-
-  Definition close_scope (stack : t) : t + string :=
-    match stack with
-    | [] => inr "cannot close the last scope as there are none left"
-    | _ :: stack => inl stack
-    end.
-
-  Fixpoint get_var (stack : t) (name : string) : U256.t + string :=
-    match stack with
-    | [] => inr ("variable '" ++ name ++ "' not found")%string
-    | locals :: stack =>
-      match Dict.get locals name with
-      | None => get_var stack name
-      | Some value => inl value
-      end
-    end.
-
-  Definition declare_var (stack : t) (name : string) (value : U256.t) : t + string :=
-    match stack with
-    | [] => inr "no scope to declare the variable"
-    | locals :: stack => inl (Dict.declare locals name value :: stack)
-    end.
-
-  Fixpoint declare_vars_aux (stack : t) (names : list string) (values : list U256.t) :
-      option (t + string) :=
-    match names, values with
-    | [], [] => Some (inl stack)
-    | name :: names, value :: values =>
-      match declare_var stack name value with
-      | inl stack => declare_vars_aux stack names values
-      | inr error => Some (inr error)
-      end
-    | _, _ => None
-    end.
-
-  Definition declare_vars (stack : t) (names : list string) (values : list U256.t) : t + string :=
-    match declare_vars_aux stack names values with
-    | Some result => result
-    | None =>
-      inr (
-        "declare: names and values have different lengths for names: " ++
-        String.concat ", " names
-      )%string
-    end.
-
-  Fixpoint assign_var (stack : t) (name : string) (value : U256.t) : t + string :=
-    match stack with
-    | [] => inr ("variable '" ++ name ++ "' not found")%string
-    | locals :: stack =>
-      match Dict.assign locals name value with
-      | None =>
-        match assign_var stack name value with
-        | inl stack => inl (locals :: stack)
-        | inr error => inr error
-        end
-      | Some locals => inl (locals :: stack)
-      end
-    end.
-
-  Fixpoint assign_vars_aux (stack : t) (names : list string) (values : list U256.t) :
-      option (t + string) :=
-    match names, values with
-    | [], [] => Some (inl stack)
-    | name :: names, value :: values =>
-      match assign_var stack name value with
-      | inl stack => assign_vars_aux stack names values
-      | inr error => Some (inr error)
-      end
-    | _, _ => None
-    end.
-
-  Definition assign_vars (stack : t) (names : list string) (values : list U256.t) : t + string :=
-    match assign_vars_aux stack names values with
-    | Some result => result
-    | None =>
-      inr (
-        "assign: names and values have different lengths for names: " ++
-        String.concat ", " names
-      )%string
-    end.
-End Stack.
-
-Module State.
-  (** The state contains the various kinds of memory that we use in a smart contract. *)
-  Record t : Set := {
-    stack : Stack.t;
-    memory : Memory.t;
-    return_data : list Z;
-    transient_storage : Storage.t;
-    accounts : list (U256.t * Account.t);
-    logs : list (list U256.t * list Z);
-    (** This is only for debugging *)
-    call_stack : CallStack.t;
+Module State(D: DIALECT).
+  (* State of the program *)
+  Module VariableAssignmentD := VariableAssignment(D).
+  Module CallStackD := CallStack(D).
+    
+  Record t : Type := {
+    variable_assignments : VariableAssignmentD.t;
+    call_stack : CallStackD.t;
+    status : Status.t;
+    dialect_state : D.dialect_state;
   }.
 
-  Definition init : State.t :=
-    {|
-      State.stack := [];
-      State.memory := Memory.empty;
-      State.return_data := [];
-      State.transient_storage := Memory.empty;
-      State.accounts := [];
-      State.logs := [];
-      State.call_stack := [];
-    |}.
+  Definition empty : t := {|
+    variable_assignments := VariableAssignmentD.empty;
+    call_stack := CallStackD.empty;
+    status := Status.Running;
+    dialect_state := D.empty_dialect_state;
+  |}.
 End State.
-
-*)
