dialect.v
@@ -17,4 +17,5 @@ Module Type DIALECT.
   Parameter equal_values: value_t -> value_t -> bool.
 
   Parameter execute_op_code : dialect_state -> opcode_t -> list (value_t) -> (dialect_state * Status.t).
+  Parameter empty_dialect_state : dialect_state.
 End DIALECT.
